HMem/Trace/TracedProgram.lean
@@ -19,14 +19,6 @@ variable {α: Type _} [Complexity.Encoding α Memory] {β: Type _} [Complexity.E
 | [] => .exit
 | p::ps => p (build ps)
 
-@[simp] def setv (dst: Source) (b: Bool): TracedProgram → TracedProgram := op (.vop (λ _ ↦ b) dst finZeroElim)
-@[simp] def setm (dst: Source) (src: Memory): TracedProgram  → TracedProgram := op (.const dst src)
-@[simp] def copyv (dst src: Source): TracedProgram  → TracedProgram := op (.vop (λ f ↦ f 0) dst (λ (_: Fin 1) ↦ src))
-@[simp] def copy (dst src: Source): TracedProgram  → TracedProgram := op (.mop .COPY dst src)
-@[simp] def move (dst src: Source): TracedProgram  → TracedProgram := op (.mop .MOVE dst src)
-@[simp] def swap (dst src: Source): TracedProgram  → TracedProgram := op (.mop .SWAP dst src)
-@[simp] def ifv (src: Source) (pos: List (TracedProgram  → TracedProgram)) (neg: TracedProgram): TracedProgram := branch (.ifTrue (λ f ↦ f 0) (λ (_: Fin 1) ↦ src)) (λ | true => build pos | false => neg)
-
 @[match_pattern] def subroutine' (dst src: Source) {γ: Type _} (_hγ: Complexity.Encoding γ Memory) {δ: Type _} (_hδ: Complexity.Encoding δ Memory)
     (fs: γ → δ) (_h: Complexity.Computable Encoding.Model fs) (next: TracedProgram): TracedProgram :=
   subroutine dst src fs next
@@ -44,9 +36,10 @@ class HasTracedProgram (p: Program) where
   tracedProgram: TracedProgram
   tracedProgramMatches: tracedProgram.toProgram = p
 
+attribute [simp] HasTracedProgram.tracedProgram
 end Trace
 
-def Program.traced (p: Program) [htp: Trace.HasTracedProgram p]: Trace.TracedProgram := htp.tracedProgram
+@[simp] def Program.traced (p: Program) [htp: Trace.HasTracedProgram p]: Trace.TracedProgram := htp.tracedProgram
 
 @[simp] theorem Program.tracedMatches (p: Program) [Trace.HasTracedProgram p]:
     p.traced.toProgram = p := Trace.HasTracedProgram.tracedProgramMatches
