HMem/Complexity/Basic.lean
@@ -2,16 +2,16 @@ import HMem.Encoding.Basic
 import HMem.Trace.TracedProgram
 import HMem.Trace.Sound
 import Complexity.Basic
+import HMem.Complexity.Def
 
 @[simp] theorem Function.HasUncurry.apply₂ (f: α → β → γ) (arg: α × β):
     (↿f) arg = f arg.fst arg.snd := rfl
 
 namespace HMem.Complexity
 
--- instance [Complexity.Encoding α Memory]: Program.HasTrace ↿(@List.cons α) where
---   program := [ .setv 0 true ]
---   hasTracedProgram := inferInstance
---   size _ := 0
---   sound | (_, _) => by simp
+instance [Complexity.Encoding α Memory]: Program.HasTrace ↿(@List.cons α) where
+  program := [ .setv 0 true ]
+  size _ := 0
+  sound | (_, _) => by simp
 
 end HMem.Complexity
